rocq-osiris/examples/proofs/spinlock_inv.v
@@ -1,0 +1,292 @@
+From iris.base_logic.lib Require Import invariants token.
+From osiris Require Import osiris.
+From osiris.proofmode Require Import proofmode.
+From osiris.stdlib Require Import Stdlib.
+From osiris.examples Require Import og_spinlock.
+
+(** * Invariant-based spinlock specification
+
+    We follow the CMRA from Iris' [spin_lock] example, where we have:
+
+    – [lock_inv γ l R]: the physical lock bit together with the user
+      resource [R] and an exclusive token; the resource lives behind [▷].
+    – [is_lock γ l R ≔ inv N (lock_inv γ l R)]: a *persistent* handle
+      handed to every caller.
+    – [locked γ ≔ token γ]: the exclusive ghost token held by the holder.
+ *)
+
+Definition spinlock_N : namespace := nroot .@ "spinlock".
+
+Section spinlock_inv_proof.
+
+Context `{!osirisGS Σ, !na_invG Σ}.
+
+(* ------------------------------------------------------------------ *)
+(* Ghost predicates *)
+
+
+(** Invariant content.  When the lock is free ([b = false]) it stores
+    [token γ ∗ ▷R]; the [▷] absorbs the later introduced by [iInv]. *)
+Definition lock_inv (γ : gname) (l : loc) (R : iProp Σ) : iProp Σ :=
+  l ↦ #true ∨ (l ↦ #false ∗ token γ ∗ ▷R).
+
+Definition is_lock (γ : gname) (l : loc) (R : iProp Σ) : iProp Σ :=
+  inv spinlock_N (lock_inv γ l R).
+
+Definition locked (γ : gname) : iProp Σ := token γ.
+
+(* ------------------------------------------------------------------ *)
+(* Specifications *)
+
+
+(* [create ()] allocates [ref false] and exposes the lock.  The caller
+   may initialise it with any [▷R] to receive [is_lock γ l R]. *)
+Definition create_spec (u : unit) (m : microvx) : iProp Σ :=
+  imp m {{ λ (l : loc), ∀ (R : iProp Σ), ▷R ={⊤}=∗ ∃ γ, is_lock γ l R }}.
+
+(* Acquiring the lock transfers ownership of [locked γ] and [▷R]. *)
+Definition acquire_spec (l : loc) (m : microvx) : iProp Σ :=
+  ∀ γ (R : iProp Σ), is_lock γ l R -∗ imp m {{ λ (_ : unit), locked γ ∗ ▷R }}.
+
+(* Releasing requires the holder to give back [locked γ] and [▷R]. *)
+Definition release_spec (l : loc) (m : microvx) : iProp Σ :=
+  ∀ γ (R : iProp Σ), is_lock γ l R -∗ locked γ -∗ ▷R -∗ imp m {{ λ (_ : unit), True }}.
+
+Instance crash_atomic {V X} :
+  thread_step.Atomic (@Crash V X).
+Proof. constructor. inversion H; subst. inversion H1. Qed.
+
+Global Instance load_atomic l :
+  thread_step.Atomic (load l).
+Proof.
+  unfold thread_step.Atomic. intros.
+
+  destruct_thread_step.
+  unfold step_load_2.
+  destruct (σ' !! l) as [ [| |] | ]; by econstructor.
+Qed.
+
+Global Instance eload_atomic η p :
+  thread_step.Atomic (eval η (ELoad (EPath p))).
+Proof.
+  simpl_eval.
+  destruct (lookup_path η p); last apply _.
+  destruct v; simpl; try (rewrite bind_crash; apply _).
+  apply _.
+Qed.
+
+Global Instance store_atomic l v :
+  thread_step.Atomic (code.store l v).
+Proof.
+  unfold thread_step.Atomic. intros.
+
+  destruct_thread_step.
+  unfold step_store_2.
+  destruct (σ !! l0) as [ [| |] | ]; by econstructor.
+Qed.
+
+Global Instance cas_atomic l seen v' :
+  thread_step.Atomic (cas l seen v').
+Proof.
+  unfold thread_step.Atomic. intros.
+
+  destruct_thread_step.
+  unfold step_cas_2.
+  destruct (σ !! l0) as [ [| |] | ]; try by econstructor.
+  destruct (phys_eq_val _ _) as [ [|] | ]; by econstructor.
+Qed.
+
+Lemma imp_store_atomic `{Encode A} (E : coPset) N η e1 e2 Ψ ζ (Φ1 : loc → _) (Φ2 : A → _) (Φ : () → _) P :
+  ↑N ⊆ E →
+  inv N P -∗
+  impure E (eval η e1) Ψ ζ Φ1 -∗
+  impure E (eval η e2) Ψ ζ Φ2 -∗
+  (▷ ∀ l x, Φ1 l -∗ Φ2 x -∗
+            ▷ P -∗
+            ∃ v, ▷ l ↦ v ∗
+                 ▷ (l ↦ #x -∗ ▷ P ∗ Φ ())) -∗
+  impure E (eval η (EStore e1 e2)) Ψ ζ Φ.
+Proof.
+  iIntros (Hsubset) "#Hinv He1 He2 Hstore".
+  simpl_eval. fold (as_loc (eval η e1)).
+  iApply (imp_bind (A1:=loc * A) with "[-]").
+  set_postcondition
+    (λ '((l, x) : loc * A),
+        |={E,E ∖ ↑N}=> ∃ v, ▷ l ↦ v ∗
+                            ▷ (l ↦ #x -∗ |={E∖↑N,E}=> Φ ()))%I.
+  { iApply (imp_Par with "[He1] He2").
+    { iApply (imp_as_loc with "He1"). }
+    iSplit.
+    - iIntros (e) "He !>". iApply (imp_throw with "He").
+    - iIntros (l x) "HΦ1 HΦ2 !>".
+      iApply imp_ret. instantiate (1:=(_,_)). encode.
+      iPoseProof (inv_acc with "Hinv") as ">[Hopen Hclose]". assumption.
+      iModIntro.
+      iDestruct ("Hstore" with "HΦ1 HΦ2 Hopen") as "(%v & $ & Hstore)".
+      iNext.
+      iIntros "Hl".
+      iDestruct ("Hstore" with "Hl") as "(HP & HΦ)".
+      iMod ("Hclose" with "HP").
+      iApply "HΦ". }
+  iIntros ((l & x)) "Hl /=".
+  iApply (imp_atomic' E (E ∖ ↑N)).
+  iMod "Hl" as "(%v & Hl & Hstore)".
+  iApply (imp_store' with "Hl").
+  iApply "Hstore".
+Qed.
+
+Lemma imp_CAS_atomic `{PhysEqDec A} N (E : coPset) η e1 e2 e3 Ψ ζ (Φ1 : loc → _) (Φ2 Φ3 : A → _) (Φ : bool → _) P :
+  ↑N ⊆ E →
+  inv N P -∗
+  impure E (eval η e1) Ψ ζ Φ1 -∗
+  impure E (eval η e2) Ψ ζ Φ2 -∗
+  impure E (eval η e3) Ψ ζ Φ3 -∗
+  (▷ ∀ l seen v',
+     Φ1 l -∗ Φ2 seen -∗ Φ3 v' -∗
+     ▷ P -∗
+     ∃ v, ▷ l ↦ #v ∗
+          ▷ (l ↦ (if phys_eq_val_ v seen then #v' else #v) -∗
+             ▷ P ∗ Φ (phys_eq_val_ v seen))) -∗
+  impure E (eval η (ECAS e1 e2 e3)) Ψ ζ Φ.
+Proof.
+  iIntros (Hsubset) "#Hinv He1 He2 He3 Hcas".
+  simpl_eval. fold (as_loc (eval η e1)).
+  iApply (imp_bind (A1:=loc * A * A) with "[-]").
+  set_postcondition
+    (λ '((l, seen, v') : loc * A * A),
+       |={E,E ∖ ↑N}=> ∃ v, ▷ l ↦ #v ∗
+       ▷ (l ↦ (if phys_eq_val_ v seen then #v' else #v) -∗ |={E ∖ ↑N,E}=> Φ (phys_eq_val_ v seen)))%I.
+  { iApply (imp_Par (A1:=loc * A) with "[He1 He2] He3").
+    { iApply (imp_Par with "[He1] He2").
+      { iApply (imp_as_loc with "He1"). }
+      iSplit.
+      - iIntros (e) "He !>". iApply (imp_throw with "He").
+      - iIntros (l x) "HΦ1 HΦ2 !>".
+        set_postcondition (λ '(l, x), Φ1 l ∗ Φ2 x)%I.
+        iApply imp_ret. instantiate (1:=(_,_)). encode.
+        iFrame. }
+    iSplit.
+    - iIntros (e) "He !>". iApply (imp_throw with "He").
+    - iIntros ((l & seen) x) "(HΦ1 & HΦ2) HΦ3".
+      iApply imp_ret. instantiate (1:=((_,_),_)). encode.
+      iNext.
+      iPoseProof (inv_acc with "Hinv") as ">[Hopen Hclose]". assumption.
+      iModIntro.
+      iDestruct ("Hcas" with "HΦ1 HΦ2 HΦ3 Hopen") as "(%v & $ & Hcas)".
+      iIntros "!> Hl".
+      iDestruct ("Hcas" with "Hl") as "(HP & HΦ)".
+      iMod ("Hclose" with "HP").
+      iApply "HΦ". }
+  iIntros (((l & seen) & x)) "Hcas /=".
+  iApply (imp_atomic' E (E ∖ ↑N)).
+  iMod "Hcas" as "(%v & Hl & Hcas)". iModIntro.
+  iApply (imp_cas with "Hl Hcas").
+Qed.
+
+(* ------------------------------------------------------------------ *)
+(* Module-level theorem *)
+
+Lemma spinlock_inv_proof :
+  ⊢ imp (eval_mexpr stdlib_env __main)
+    {{ context [
+         var_spec "create"  (λ create,  □ iSpec τ[unit] create create_spec);
+         var_spec "acquire" (λ acquire, □ iSpec τ[loc]  acquire acquire_spec);
+         var_spec "release" (λ release, □ iSpec τ[loc]  release release_spec)
+       ] {["create"; "acquire"; "release"]} }}.
+Proof.
+  iApply imp_module.
+
+  (* ------------------------------------------------------------------ *)
+  (* Subgoal: [let create () = ref false] *)
+
+  iApply (imp_sitems_let (λ create : val, □ iSpec τ[unit] create create_spec)%I).
+  { iApply (imp_EAnon_pers τ[unit]).
+    iIntros "!>" ([]).
+    iApply imp_please; iNext.
+    iApply (imp_EMatch (A':=unit)).
+    { imp_path. }
+    iIntros (? ->) "!>".
+    iApply deep_handle_cons.
+    { iPureIntro; ltac2:(let _ := specify_cpattern () in ()). pattern_match. apply eq_refl. }
+    iSplit; last iIntros ([]).
+    iIntros (?) "<-".
+    (* After [ref false] we have [l ↦ #false]; use it to build the invariant. *)
+    iApply (imp_wand).
+    { imp_ref false. }
+    iIntros (l) "Hl".
+    (* Goal: ∀ R, ▷R ={⊤}=∗ ∃ γ, is_lock γ l R *)
+    iIntros (R) "HR".
+    iMod token_alloc as "(%γ & Htok)".
+    iMod (inv_alloc spinlock_N _ (lock_inv γ l R) with "[Hl Htok HR]") as "#Hinv".
+    { (* Provide ▷ (lock_inv γ l R) with b = false via [later_intro]. *)
+      iNext. iRight. iFrame. }
+    iModIntro. iExists γ. iExact "Hinv". }
+
+  iIntros (create) "#Hcreate".
+
+  (* ------------------------------------------------------------------ *)
+  (* Subgoal: [let acquire lk = while !lk do () done; lk := true] *)
+
+  iApply (imp_sitems_let (λ acquire : val, □ iSpec τ[loc] acquire acquire_spec)%I).
+  { iApply (imp_EAnon_pers τ[loc]).
+    (* After introducing [l : loc], the spec universally quantifies over [γ] and
+       [R]; we introduce them here. *)
+    iIntros "!>" (l). unfold acquire_spec.
+    iIntros (γ R) "#Hinv".
+    iApply imp_please; iNext.
+
+    (* Subgoal: [while not (Atomic.set_and_compare lk false true) do () done] *)
+    iApply (imp_EWhile (λ b, if b then True else locked γ ∗ ▷ R)%I).
+    - (* I true *)
+      done.
+    - (* Condition: load [!lk] directly from [l ↦ #b'] *)
+      iIntros "!> _".
+      iApply imp_EBoolNeg.
+
+      iApply (imp_CAS_atomic (A:=bool) with "Hinv"); try imp_step. set_solver.
+      iIntros "!>" (???) "-> -> -> [Hl | (Hl & Htok & HR) ]".
+
+      + (* Subcase: the CAS returned true. *)
+        iFrame.
+        iIntros "!> Hl".
+        iSplitL. { iLeft. iApply "Hl". } done.
+
+      + (* Subcase: the CAS returned false. *)
+        iFrame.
+        iIntros "!> Hl".
+        simpl. iFrame.
+
+    - (* Evaluating the body. *)
+      iIntros "!> _".
+      by iApply imp_EUnit. }
+
+  iIntros (acquire) "#Hacquire".
+
+  (* ------------------------------------------------------------------ *)
+  (* Subgoal: [let release lk = lk := false] *)
+  iApply (imp_sitems_let (λ release : val, □ iSpec τ[loc] release release_spec)%I).
+  { iApply (imp_EAnon_pers τ[loc]).
+    iIntros "!>" (l).
+    iIntros (γ R) "#Hinv Htok HR".
+    iApply imp_please; iNext.
+    (* Open invariant non-atomically: get [l ↦ #b] in hand, store [false],
+       then close with [l ↦ #false ∗ token γ ∗ ▷R]. *)
+    iApply (imp_store_atomic (A:=bool) with "Hinv"); try imp_step. set_solver.
+    iIntros "!>" (??) "-> -> Hopened".
+    iDestruct "Hopened" as "[ $ | ($ & >Htok' & HR') ]".
+    - iIntros "!> Hl".
+      iSplitL. { iRight. iFrame. }
+      done.
+    - (* This case is impossible: we own [token γ],
+         so the lock cannot have been open. *)
+      iPoseProof (token_exclusive with "Htok Htok'") as "[]". }
+
+  iIntros (release) "#Hrelease".
+
+  (* ------------------------------------------------------------------ *)
+  (* Conclude                                                            *)
+  iApply imp_sitems_nil.
+  iFrame "#"; simpl. auto.
+Qed.
+
+End spinlock_inv_proof.
